Spec for DH

specs/ecdsap256sha2/Hacl.Spec.DH.fst
@@ -3,6 +3,7 @@ module Hacl.Spec.DH
 open Lib.IntTypes
 open Lib.Buffer
 open Lib.ByteSequence
+open Lib.Sequence
 
 open FStar.Mul
 open FStar.Math.Lemmas
@@ -10,13 +11,33 @@ open FStar.Math.Lemmas
 open Hacl.Spec.P256
 open Hacl.Spec.P256.Definitions
 
+open Hacl.Spec.ECDSA
+
+#set-options "--fuel 0 --ifuel 0 --z3rlimit 300"
 (* the code for initiator of DH key exchange *)
 
-val ecp256_dh_i: s: lbytes 32 -> Tot (tuple3 (xN: nat {xN < prime256}) (yN: nat {yN < prime256}) (uint64)) 
+val ecp256_dh_i: s: lbytes 32 -> Tot (r: tuple3 (lbytes 32) (lbytes 32) uint64)
 
 let ecp256_dh_i s = 
   let xN, yN, zN = secret_to_public s in 
   if isPointAtInfinity (xN, yN, zN) then 
-    xN, yN, u64 (pow2 64 - 1)
+    nat_to_bytes_be #SEC 32 xN, nat_to_bytes_be #SEC 32 yN, u64 (pow2 64 - 1)
   else 
-    xN, yN, u64 0
+    nat_to_bytes_be #SEC 32 xN, nat_to_bytes_be #SEC 32 yN, (u64 0)
+
+(* the code for repondeur of DH key exchange *)
+
+
+val ecp256_dh_r: x: lbytes 32 -> y: lbytes 32 -> s: lbytes 32 -> Tot (tuple3 (lbytes 32) (lbytes 32) uint64)
+
+let ecp256_dh_r x y s = 
+  let x_, y_ = nat_from_bytes_be x, nat_from_bytes_be y in 
+  let pointJacX, pointJacY, pointJacZ = toJacobianCoordinates (x_, y_) in 
+  if not (verifyQValidCurvePointSpec (pointJacX, pointJacY, pointJacZ)) then 
+    nat_to_bytes_be #SEC 32 0, nat_to_bytes_be #SEC 32 0, u64 (pow2 64 - 1)
+  else
+    let xN, yN, zN = scalar_multiplication s (pointJacX, pointJacY, pointJacZ) in 
+    if isPointAtInfinity (xN, yN, zN) then
+      nat_to_bytes_be #SEC 32 xN, nat_to_bytes_be #SEC 32 yN, u64 (pow2 64 - 1)
+    else 
+      nat_to_bytes_be #SEC 32 xN, nat_to_bytes_be #SEC 32 yN, u64 0
